perf: optimize Nat.Linear.Poly.norm (#6064)
Not a huge benefit, but actually reduces the code complexity (no need
for the `.fuse` function), and can help with problems with many repeated
varibles.

src/Init/Data/Nat/Linear.lean
@@ -52,25 +52,23 @@ def Poly.denote (ctx : Context) (p : Poly) : Nat :=
   | [] => 0
   | (k, v) :: p => Nat.add (Nat.mul k (v.denote ctx)) (denote ctx p)
 
-def Poly.insertSorted (k : Nat) (v : Var) (p : Poly) : Poly :=
+def Poly.insert (k : Nat) (v : Var) (p : Poly) : Poly :=
   match p with
   | [] => [(k, v)]
-  | (k', v') :: p => bif Nat.blt v v' then (k, v) :: (k', v') :: p else (k', v') :: insertSorted k v p
+  | (k', v') :: p =>
+    bif Nat.blt v v' then
+      (k, v) :: (k', v') :: p
+    else bif Nat.beq v v' then
+      (k + k', v') :: p
+    else
+      (k', v') :: insert k v p
 
-def Poly.sort (p : Poly) : Poly :=
-  let rec go (p : Poly) (r : Poly) : Poly :=
+def Poly.norm (p : Poly) : Poly := go p []
+where
+  go (p : Poly) (r : Poly) : Poly :=
     match p with
     | [] => r
-    | (k, v) :: p => go p (r.insertSorted k v)
-  go p []
-
-def Poly.fuse (p : Poly) : Poly :=
-  match p with
-  | []  => []
-  | (k, v) :: p =>
-    match fuse p with
-    | [] => [(k, v)]
-    | (k', v') :: p' => bif v == v' then (Nat.add k k', v)::p' else (k, v) :: (k', v') :: p'
+    | (k, v) :: p => go p (r.insert k v)
 
 def Poly.mul (k : Nat) (p : Poly) : Poly :=
   bif k == 0 then
@@ -146,7 +144,8 @@ def Poly.combineAux (fuel : Nat) (p₁ p₂ : Poly) : Poly :=
 def Poly.combine (p₁ p₂ : Poly) : Poly :=
   combineAux hugeFuel p₁ p₂
 
-def Expr.toPoly (e : Expr) := go 1 e []
+def Expr.toPoly (e : Expr) :=
+  go 1 e []
 where
   -- Implementation note: This assembles the result using difference lists
   -- to avoid `++` on lists.
@@ -156,9 +155,6 @@ where
     | Expr.add a b  => go coeff a ∘ go coeff b
     | Expr.mulL k a
     | Expr.mulR a k => bif k == 0 then id else go (coeff * k) a
-
-def Poly.norm (p : Poly) : Poly :=
-  p.sort.fuse
 
 def Expr.toNormPoly (e : Expr) : Poly :=
   e.toPoly.norm
@@ -205,7 +201,7 @@ def PolyCnstr.denote (ctx : Context) (c : PolyCnstr) : Prop :=
     Poly.denote_le ctx (c.lhs, c.rhs)
 
 def PolyCnstr.norm (c : PolyCnstr) : PolyCnstr :=
-  let (lhs, rhs) := Poly.cancel c.lhs.sort.fuse c.rhs.sort.fuse
+  let (lhs, rhs) := Poly.cancel c.lhs.norm c.rhs.norm
   { eq := c.eq, lhs, rhs }
 
 def PolyCnstr.isUnsat (c : PolyCnstr) : Bool :=
@@ -272,24 +268,32 @@ def PolyCnstr.toExpr (c : PolyCnstr) : ExprCnstr :=
   { c with lhs := c.lhs.toExpr, rhs := c.rhs.toExpr }
 
 attribute [local simp] Nat.add_comm Nat.add_assoc Nat.add_left_comm Nat.right_distrib Nat.left_distrib Nat.mul_assoc Nat.mul_comm
-attribute [local simp] Poly.denote Expr.denote Poly.insertSorted Poly.sort Poly.sort.go Poly.fuse Poly.cancelAux
+attribute [local simp] Poly.denote Expr.denote Poly.insert Poly.norm Poly.norm.go Poly.cancelAux
 attribute [local simp] Poly.mul Poly.mul.go
 
-theorem Poly.denote_insertSorted (ctx : Context) (k : Nat) (v : Var) (p : Poly) : (p.insertSorted k v).denote ctx = p.denote ctx + k * v.denote ctx := by
+theorem Poly.denote_insert (ctx : Context) (k : Nat) (v : Var) (p : Poly) :
+    (p.insert k v).denote ctx = p.denote ctx + k * v.denote ctx := by
   match p with
   | [] => simp
-  | (k', v') :: p => by_cases h : Nat.blt v v' <;> simp [h, denote_insertSorted]
+  | (k', v') :: p =>
+    by_cases h₁ : Nat.blt v v'
+    · simp [h₁]
+    · by_cases h₂ : Nat.beq v v'
+      · simp only [insert, h₁, h₂, cond_false, cond_true]
+        simp [Nat.eq_of_beq_eq_true h₂]
+      · simp only [insert, h₁, h₂, cond_false, cond_true]
+        simp [denote_insert]
 
-attribute [local simp] Poly.denote_insertSorted
+attribute [local simp] Poly.denote_insert
 
-theorem Poly.denote_sort_go (ctx : Context) (p : Poly) (r : Poly) : (sort.go p r).denote ctx = p.denote ctx + r.denote ctx := by
+theorem Poly.denote_norm_go (ctx : Context) (p : Poly) (r : Poly) : (norm.go p r).denote ctx = p.denote ctx + r.denote ctx := by
   match p with
   | [] => simp
-  | (k, v):: p => simp [denote_sort_go]
+  | (k, v):: p => simp [denote_norm_go]
 
-attribute [local simp] Poly.denote_sort_go
+attribute [local simp] Poly.denote_norm_go
 
-theorem Poly.denote_sort (ctx : Context) (m : Poly) : m.sort.denote ctx = m.denote ctx := by
+theorem Poly.denote_sort (ctx : Context) (m : Poly) : m.norm.denote ctx = m.denote ctx := by
   simp
 
 attribute [local simp] Poly.denote_sort
@@ -319,18 +323,6 @@ theorem Poly.denote_reverse (ctx : Context) (p : Poly) : denote ctx (List.revers
   simp [List.reverse]
 
 attribute [local simp] Poly.denote_reverse
-
-theorem Poly.denote_fuse (ctx : Context) (p : Poly) : p.fuse.denote ctx = p.denote ctx := by
-  match p with
-  | [] => rfl
-  | (k, v) :: p =>
-    have ih := denote_fuse ctx p
-    simp
-    split
-    case _ h => simp [← ih, h]
-    case _ k' v' p' h => by_cases he : v == v' <;> simp [he, ← ih, h]; rw [eq_of_beq he]
-
-attribute [local simp] Poly.denote_fuse
 
 theorem Poly.denote_mul (ctx : Context) (k : Nat) (p : Poly) : (p.mul k).denote ctx = k * p.denote ctx := by
   simp
